better notation

Semantics/Imp/Aexp.lean
@@ -3,17 +3,25 @@ import Semantics.Imp.Lang
 namespace Aexp
 namespace Natural
 
-inductive step: Aexp → State → Int → Prop
-  | valₙ: step (val₁ n) _ n
-  | varₙ: step (var₁ x) s (s x)
-  | addₙ (ha: step a s n) (hb: step b s m):
-    step (a + b) s (n + m)
-  | subₙ (ha: step a s n) (hb: step b s m):
-    step (a - b) s (n - m)
-  | mulₙ (ha: step a s n) (hb: step b s m):
-    step (a * b) s (n * m)
+private inductive step: Aexp × State → Int → Prop
+  | valₙ: step (val₁ n, _) n
+  | varₙ: step (var₁ x, s) (s x)
+  | addₙ (ha: step (a, s) n) (hb: step (b, s) m):
+    step (a + b, s) (n + m)
+  | subₙ (ha: step (a, s) n) (hb: step (b, s) m):
+    step (a - b, s) (n - m)
+  | mulₙ (ha: step (a, s) n) (hb: step (b, s) m):
+    step (a * b, s) (n * m)
 
-notation s " ⊢ " a " ⟹ " v => step a s v
+infixl:10 " ⟹ₐ " => step
+
+private instance step.equiv: Setoid Aexp where
+  r a b := ∀s n, ((a, s) ⟹ₐ n) = ((b, s) ⟹ₐ n)
+  iseqv := {
+    refl := λ _ _ _ => rfl
+    symm := λ h s n => (h s n).symm
+    trans := λ h1 h2 s n => (h1 s n) ▸ (h2 s n)
+  }
 
 end Natural
 
@@ -25,17 +33,28 @@ def reduce (a: Aexp) (s: State): Int :=
   | sub₁ a b => reduce a s - reduce b s
   | mul₁ a b => reduce a s * reduce b s
 
-infix:100 "⇓" => reduce
+instance: CoeFun Aexp (λ _ => State → Int) where
+  coe a := reduce a
+
+instance reduce.equiv: Setoid Aexp where
+  r a b := ∀s, a s = b s
+  iseqv := {
+    refl := λ _ _ => rfl
+    symm := λ h s => (h s).symm
+    trans := λ h1 h2 s => (h1 s) ▸ (h2 s)
+  }
+
+section Equivalence
 
 -- relational definition is equal to recursive
-theorem reduce.from_natural (h: s ⊢ a ⟹ n): a⇓s = n :=
+private theorem reduce.from_natural (h: p ⟹ₐ n): p.1 p.2 = n :=
   by induction h with
   | addₙ _ _ iha ihb => exact iha ▸ ihb ▸ rfl
   | subₙ _ _ iha ihb => exact iha ▸ ihb ▸ rfl
   | mulₙ _ _ iha ihb => exact iha ▸ ihb ▸ rfl
   | _ => rfl
 
-theorem Natural.from_reduce {a: Aexp} (h: a⇓s = n): s ⊢ a ⟹ n :=
+private theorem Natural.from_reduce {a: Aexp} (h: a s = n): (a, s) ⟹ₐ n :=
   by induction a generalizing n with
   | val₁ a => exact h ▸ step.valₙ
   | var₁ a => exact h ▸ step.varₙ
@@ -43,39 +62,25 @@ theorem Natural.from_reduce {a: Aexp} (h: a⇓s = n): s ⊢ a ⟹ n :=
   | sub₁ a b iha ihb => exact h ▸ step.subₙ (iha rfl) (ihb rfl)
   | mul₁ a b iha ihb => exact h ▸ step.mulₙ (iha rfl) (ihb rfl)
 
-theorem step_eq_reduce: (s ⊢ a ⟹ n) = (a⇓s = n) :=
+private theorem step_eq_reduce: ((a, s) ⟹ₐ n) = (a s = n) :=
   propext ⟨reduce.from_natural, Natural.from_reduce⟩
 
-theorem step_eq_reduce': s ⊢ a ⟹ (a⇓s) :=
+private theorem step_eq_reduce': (a, s) ⟹ₐ a s :=
   Natural.from_reduce rfl
 
-protected instance step.equiv: Setoid Aexp where
-  r a b := ∀s n, (s ⊢ a ⟹ n) = (s ⊢ b ⟹ n)
-  iseqv := {
-    refl := λ _ _ _ => rfl
-    symm := λ h s n => (h s n).symm
-    trans := λ h1 h2 s n => (h1 s n) ▸ (h2 s n)
-  }
-
-instance reduce.equiv: Setoid Aexp where
-  r a b := ∀s, a⇓s = b⇓s
-  iseqv := {
-    refl := λ _ _ => rfl
-    symm := λ h s => (h s).symm
-    trans := λ h1 h2 s => (h1 s) ▸ (h2 s)
-  }
-
-protected theorem step_eq_eq_reduce_eq:
-  step.equiv.r a b ↔ reduce.equiv.r a b := by
+private theorem step_eq_eq_reduce_eq:
+  Natural.step.equiv.r a b ↔ reduce.equiv.r a b := by
   simp only [Setoid.r, eq_iff_iff]
   constructor
   . intro h s
-    specialize h s (b⇓s)
+    specialize h s $ b s
     rw [step_eq_reduce, step_eq_reduce, eq_self, iff_true] at h
     exact h
   . intro h s _
     rw [step_eq_reduce, step_eq_reduce]
     specialize h s
     rw [h]
+
+end Equivalence
 
 end Aexp
