Semantics/Imp/Bexp.lean
@@ -4,19 +4,27 @@ namespace Bexp
 namespace Natural
 
 -- Operational semantics of Bexp
-inductive step: Bexp → State → Bool → Prop
-  | trueₙ: step true₁ _ true
-  | falseₙ: step false₁ _ false
-  | notₙ (h: step a s n):
-    step (!a) s (!n)
-  | andₙ (h₁: step a s n) (h₂: step b s m):
-    step (a && b) s (n && m)
-  | orₙ (h₁: step a s n) (h₂: step b s m):
-    step (a || b) s (n || m)
-  | eqₙ: step (a == b) s (a⇓s == b⇓s)
-  | leₙ: step (a <= b) s (a⇓s <= b⇓s)
+private inductive step: Bexp × State → Bool → Prop
+  | trueₙ: step (true₁, _) true
+  | falseₙ: step (false₁, _) false
+  | notₙ (h: step (a, s) n):
+    step (~~~a, s) (!n)
+  | andₙ (h₁: step (a, s) n) (h₂: step (b, s) m):
+    step (a &&& b, s) (n && m)
+  | orₙ (h₁: step (a, s) n) (h₂: step (b, s) m):
+    step (a ||| b, s) (n || m)
+  | eqₙ: step (eq₁ a b, s) (a s == b s)
+  | leₙ: step (le₁ a b, s) (a s <= b s)
 
-notation s " ⊢ " b " ⟹ " v => step b s v
+infixl:10 " ⟹ₗ " => step
+
+private instance step.equiv: Setoid Bexp where
+  r a b := ∀s n, ((a, s) ⟹ₗ n) = ((b, s) ⟹ₗ n)
+  iseqv := {
+    refl := λ _ _ _ => rfl
+    symm := λ h s n => (h s n).symm
+    trans := λ h1 h2 s n => (h1 s n) ▸ (h2 s n)
+  }
 
 end Natural
 
@@ -31,10 +39,30 @@ def reduce (b: Bexp) (s: State): Bool :=
   | eq₁ a b  => a.reduce s == b.reduce s
   | le₁ a b  => a.reduce s <= b.reduce s
 
-infix:100 "⇓" => reduce
+instance: CoeFun Bexp (λ _ => State → Bool) where
+  coe b := reduce b
+
+instance reduce.equiv: Setoid Bexp where
+  r a b:= ∀s, a s = b s
+  iseqv := {
+    refl := λ _ _ => rfl
+    symm := λ h s => (h s).symm
+    trans := λ h1 h2 s => (h1 s) ▸ (h2 s)
+  }
+
+section Equivalence
 
 -- relational definition is equivalent to recursive
-theorem Natural.from_reduce {b: Bexp} (h: b⇓s = x): s ⊢ b ⟹ x :=
+private theorem reduce.from_natural {p: Bexp × State}
+  (h: p ⟹ₗ x): p.1 p.2 = x :=
+  by induction h with
+  | notₙ _ ih => exact ih ▸ rfl
+  | andₙ _ _ iha ihb => exact iha ▸ ihb ▸ rfl
+  | orₙ _ _ iha ihb => exact iha ▸ ihb ▸ rfl
+  | _ => rfl
+
+private theorem Natural.from_reduce {b: Bexp}
+  (h: b s = x): (b, s) ⟹ₗ x :=
   by induction b generalizing x with
   | true₁ => exact h ▸ step.trueₙ
   | false₁ => exact h ▸ step.falseₙ
@@ -44,48 +72,27 @@ theorem Natural.from_reduce {b: Bexp} (h: b⇓s = x): s ⊢ b ⟹ x :=
   | eq₁ => exact h ▸ step.eqₙ
   | le₁ => exact h ▸ step.leₙ
 
-theorem reduce.from_natural {b: Bexp} (h: s ⊢ b ⟹ x): b⇓s = x :=
-  by induction h with
-  | notₙ _ ih => exact ih ▸ rfl
-  | andₙ _ _ iha ihb => exact iha ▸ ihb ▸ rfl
-  | orₙ _ _ iha ihb => exact iha ▸ ihb ▸ rfl
-  | _ => rfl
-
-theorem step_eq_reduce {b: Bexp}: (s ⊢ b ⟹ x) = (b⇓s = x) :=
+private theorem step_eq_reduce {b: Bexp}: ((b, s) ⟹ₗ x) = (b s = x) :=
   propext ⟨reduce.from_natural, Natural.from_reduce⟩
 
-theorem step_eq_reduce' {b: Bexp}: s ⊢ b ⟹ (b⇓s) :=
+private theorem step_eq_reduce' {b: Bexp}: (b, s) ⟹ₗ b s :=
   Natural.from_reduce rfl
 
-theorem not_true_eq_false: (!b⇓s) = (!b)⇓s := rfl
+private theorem not_true_eq_false: (!(reduce b s)) = (~~~b) s := rfl
 
-protected instance step.equiv: Setoid Bexp where
-  r a b := ∀ s n, Natural.step a s n = Natural.step b s n
-  iseqv := {
-    refl := λ _ _ _ => rfl
-    symm := λ h s n => (h s n).symm
-    trans := λ h1 h2 x n => (h1 x n) ▸ (h2 x n)
-  }
-
-instance reduce.equiv: Setoid Bexp where
-  r a b:= ∀s, a⇓s = b⇓s
-  iseqv := {
-    refl := λ _ _ => rfl
-    symm := λ h s => (h s).symm
-    trans := λ h1 h2 s => (h1 s) ▸ (h2 s)
-  }
-
-protected theorem step_eq_eq_reduce_eq:
-  step.equiv.r a b ↔ reduce.equiv.r a b := by
+private theorem step_eq_eq_reduce_eq:
+  Natural.step.equiv.r a b ↔ reduce.equiv.r a b := by
   simp only [Setoid.r, eq_iff_iff]
   constructor
   . intro h s
-    exact (step_eq_reduce ▸ h s (b⇓s)).mpr $ step_eq_reduce.mpr rfl
+    exact (step_eq_reduce ▸ h s (b s)).mpr $ step_eq_reduce.mpr rfl
   . intro h s _
     constructor
     . intro h1
       exact ((h s) ▸ (step_eq_reduce ▸ h1)) ▸ step_eq_reduce'
     . intro h1
       exact ((h s) ▸ (step_eq_reduce ▸ h1)) ▸ step_eq_reduce'
+
+end Equivalence
 
 end Bexp
