Semantics/Imp/Natural.lean
@@ -3,89 +3,92 @@ import Semantics.Imp.Bexp
 namespace Com
 namespace Natural
 
-inductive step: Com → State → State → Prop
+inductive step: Com × State → State → Prop
   | skipₙ:
-    step skip₁ s s
+    step (skip₁, s) s
 
   | assₙ:
-    step (x = a) s (s⟪x ≔ a⇓s⟫)
+    step (ass₁ x a, s) (s[x ← a s])
 
-  | catₙ (t: State) (hc: step c s t) (hd: step d t u):
-    step (c;;d) s u
+  | catₙ (t: State) (hc: step (c, s) t) (hd: step (d, t) u):
+    step (c++d, s) u
 
-  | if₀ₙ {b: Bexp} (hb: b⇓s = false) (hd: step d s t):
-    step if b then c else d end s t
+  | if₀ₙ {b: Bexp} (hb: b s = false) (hd: step (d, s) t):
+    step (if b then c else d end, s) t
 
-  | if₁ₙ {b: Bexp} (hb: b⇓s = true) (hc: step c s t):
-    step if b then c else d end s t
+  | if₁ₙ {b: Bexp} (hb: b s = true) (hc: step (c, s) t):
+    step (if b then c else d end, s) t
 
-  | while₀ₙ {b: Bexp} (hb: b⇓s = false):
-    step while b loop c end s s
+  | while₀ₙ {b: Bexp} (hb: b s = false):
+    step (while b loop c end, s) s
 
-  | while₁ₙ {b: Bexp} (u: State) (hb: b⇓s = true) (hc: step c s u)
-    (hw: step while b loop c end u t):
-    step while b loop c end s t
+  | while₁ₙ {b: Bexp} (u: State) (hb: b s = true) (hc: step (c, s) u)
+    (hw: step (while b loop c end, u) t):
+    step (while b loop c end, s) t
 
-notation:10 s " ⊢ " c " ⟹ " t => step c s t
+infixl:10 " ⟹ " => step
 
-private def x := "x"
-private def z := "z"
+private example: (⦃x = 5⦄, s₀) ⟹ (s₀["x" ← 5]) := step.assₙ
 
-private example: σ₀ ⊢ ⦃x = 5⦄ ⟹ σ₀⟪x ≔ 5⟫ := step.assₙ
 private example:
-  σ₀ ⊢ ⦃x = 2; if x <= 1 then y = 3 else z = 4 end⦄ ⟹ σ₀⟪x ≔ 2⟫⟪z ≔ 4⟫ :=
+   (⦃x = 2; if x <= 1 then y = 3 else z = 4 end⦄, s₀)
+    ⟹ s₀["x" ← 2]["z" ← 4] :=
     step.catₙ _ step.assₙ $ step.if₀ₙ rfl step.assₙ
+
 private example:
-  σ₀ ⊢ ⦃x = 2; x = 3⦄ ⟹ σ₀⟪x ≔ 3⟫ :=
-  let h1: σ₀⟪x ≔ 3⟫ = σ₀⟪x ≔ 2⟫⟪x ≔ 3⟫ := TotalMap.clobber.symm
+  (⦃x = 2; x = 3⦄, s₀) ⟹ s₀["x" ← 3] :=
+  let h1: s₀["x" ← 3] = s₀["x" ← 2]["x" ← 3] := TotalMap.clobber.symm
   h1 ▸ step.catₙ _ step.assₙ step.assₙ
 
 /-
 ## Rewriting rules
 -/
 
-theorem skip_eq: (s ⊢ skip₁ ⟹ t) = (s = t) :=
+theorem skip_eq: ((skip₁, s) ⟹ t) = (s = t) :=
   propext {
     mp := λ (step.skipₙ) => rfl,
     mpr := (· ▸ step.skipₙ)
   }
 
 theorem cat_eq:
-  (s ⊢ c;;d ⟹ t) = ∃ w, (s ⊢ c ⟹ w) ∧ (w ⊢ d ⟹ t) :=
+  ((c++d, s) ⟹ t) = ∃ w, ((c, s) ⟹ w) ∧ ((d, w) ⟹ t) :=
   propext {
     mp := λ (step.catₙ t h1 h2) => ⟨t, h1, h2⟩,
     mpr := λ ⟨w, h1, h2⟩ => step.catₙ w h1 h2
   }
 
 theorem if_eq:
-  (s ⊢ if b then c else d end ⟹ t)
-    = bif b⇓s then (s ⊢ c ⟹ t) else (s ⊢ d ⟹ t) :=
+  ((if b then c else d end, s) ⟹ t)
+    = bif b s then (c, s) ⟹ t else (d, s) ⟹ t :=
   propext {
     mp := λ h => match h with
       | step.if₁ₙ hb h | step.if₀ₙ hb h => hb ▸ h,
-    mpr := match hb: b⇓s with
+    mpr := match hb: b s with
       | true => λ h => step.if₁ₙ hb h
       | false => λ h => step.if₀ₙ hb h
   }
 
 theorem if_eq':
-  (s ⊢ if b then c else d end ⟹ t)
-    = (s ⊢ bif b⇓s then c else d ⟹ t) :=
+  ((if b then c else d end, s) ⟹ t)
+    = ((bif b s then c else d, s) ⟹ t) :=
   propext $ {
     mp := λ h => match h with
       | step.if₁ₙ hb h | step.if₀ₙ hb h => hb ▸ h,
-    mpr := match hb: b⇓s with
+    mpr := match hb: b s with
       | true => λ h => step.if₁ₙ hb h
       | false => λ h => step.if₀ₙ hb h
   }
 
-theorem while_eq: (s ⊢ while b loop c end ⟹ t) =
-  bif b⇓s then ∃w, (s ⊢ c ⟹ w) ∧ (w ⊢ while b loop c end ⟹ t) else s = t :=
+theorem while_eq: ((while b loop c end, s) ⟹ t) =
+  bif b s then
+    ∃w, ((c, s) ⟹ w) ∧ ((while b loop c end, w) ⟹ t)
+  else
+    s = t :=
   propext {
     mp := λ h => match h with
       | step.while₁ₙ t hb hc hw => hb ▸ ⟨t, hc, hw⟩
       | step.while₀ₙ hb => hb ▸ rfl,
-    mpr := match hb: b⇓s with
+    mpr := match hb: b s with
       | true => λ ⟨w, h1, h2⟩ => step.while₁ₙ w hb h1 h2
       | false => λ h => h ▸ step.while₀ₙ hb
   }
@@ -95,20 +98,20 @@ theorem while_eq: (s ⊢ while b loop c end ⟹ t) =
 -/
 
 instance equiv: Setoid Com where
-  r c d := ∀s t, (s ⊢ c ⟹ t) ↔ (s ⊢ d ⟹ t)
+  r c d := ∀s t, ((c, s) ⟹ t) ↔ ((d, s) ⟹ t)
   iseqv := {
     refl := λ _ _ _ => Iff.rfl
     symm := (Iff.symm $ · · ·)
     trans := λ h1 h2 x n => Iff.trans (h1 x n) (h2 x n)
   }
 
-theorem skipl: (skip₁;;c) ≈ c := λ _ _ =>
+theorem skipl: (skip₁++c) ≈ c := λ _ _ =>
   {
     mp := λ (step.catₙ _ hc hd) => skip_eq.mp hc ▸ hd,
     mpr := λ h => step.catₙ _ step.skipₙ h
   }
 
-theorem skipr: (c;;skip₁) ≈ c := λ _ _ =>
+theorem skipr: (c++skip₁) ≈ c := λ _ _ =>
   {
     mp := λ (step.catₙ _ hc hd) => skip_eq.mp hd ▸ hc,
     mpr := λ h => step.catₙ _ h step.skipₙ
@@ -128,7 +131,7 @@ theorem cond_false (h: b ≈ Bexp.false₁):
 
 theorem loop_unfold:
   while b loop c end ≈
-    if b then (c;;while b loop c end) else skip₁ end := by
+    if b then (c++while b loop c end) else skip₁ end := by
   intro s t
   rw [if_eq']
   constructor
@@ -136,7 +139,7 @@ theorem loop_unfold:
     match h with
     | step.while₁ₙ w hb hc hw => exact hb ▸ step.catₙ w hc hw
     | step.while₀ₙ hb => exact hb ▸ step.skipₙ
-  . match hb: b⇓s with
+  . match hb: b s with
     | false =>
       intro (step.skipₙ)
       exact step.while₀ₙ hb
@@ -149,9 +152,9 @@ theorem loop_unfold:
 -/
 
 theorem loop_tt (h: b ≈ Bexp.true₁):
-  ¬(s ⊢ while b loop c end ⟹ t) := λ h1 => by
-  generalize h2: while b loop c end = ww at h1
-  induction h1 with
+  ¬((while b loop c end, s) ⟹ t) := λ h1 => by
+  generalize h2: (while b loop c end, s) = p at h1
+  induction h1 generalizing s with
   | while₁ₙ _ _ _ _ _ ih2 =>
     match h2 with
     | Eq.refl _ => exact ih2 rfl
@@ -160,14 +163,16 @@ theorem loop_tt (h: b ≈ Bexp.true₁):
     | Eq.refl _ =>
       rw [h] at hb
       contradiction
-  | _ => contradiction
+  | _ =>
+    match Prod.mk.injEq _ _ _ _ ▸ h2 with
+    | ⟨_, _⟩ => contradiction
 
 /-
 ## Determinism
 -/
 
-theorem deterministic {c: Com}
-  (h1: w ⊢ c ⟹ s) (h2: w ⊢ c ⟹ t): s = t :=
+theorem deterministic
+  (h1: p ⟹ s) (h2: p ⟹ t): s = t :=
   by induction h1 generalizing t with
   | skipₙ => match h2 with | step.skipₙ => rfl
   | assₙ => match h2 with | step.assₙ => rfl
