Semantics/Imp/Structural.lean
@@ -6,30 +6,31 @@ namespace Structural
 
 inductive step: Com × State → Com × State → Prop where
   | assₛ:
-    step (x = a, s) (skip₁, s⟪x ≔ a⇓s⟫)
+    step (ass₁ x a, s) (skip₁, s[x ← a s])
 
   | cat₀ₛ:
-    step (skip₁;;c, s) (c, s)
+    step (skip₁++c, s) (c, s)
 
   | catₙₛ (h: step (c, s) (e, t)):
-    step (c;;d, s) (e;;d, t)
+    step (c++d, s) (e++d, t)
 
   | ifₛ:
-    step (if b then c else d end, s) (bif b⇓s then c else d, s)
+    step (if b then c else d end, s) (bif b s then c else d, s)
 
   | whileₛ:
-    step (while b loop c end, s) (bif b⇓s then c;;while b loop c end else skip₁, s)
+    step (while b loop c end, s)
+          (bif b s then c++while b loop c end else skip₁, s)
 
-infix:110 " ⇒ " => step
+infixl:10 " ⇒ " => step
 
 private example:
-  (⦃x = 0; while x <= 2 loop x = x + 1 end⦄, σ₀) ⇒
-      (⦃skip; while x <= 2 loop x = x + 1 end⦄, σ₀⟪"x" ≔ 0⟫) :=
+  (⦃x = 0; while x <= 2 loop x = x + 1 end⦄, s₀) ⇒
+      (⦃skip; while x <= 2 loop x = x + 1 end⦄, s₀["x" ← 0]) :=
   step.catₙₛ step.assₛ
 
 theorem cat_eq:
-  (c₁;;c₂, s) ⇒ et
-    = ((∃e t, (c₁, s) ⇒ (e, t) ∧ et = (e;;c₂, t))
+  ((c₁++c₂, s) ⇒ et)
+    = ((∃e t, ((c₁, s) ⇒ (e, t)) ∧ et = (e++c₂, t))
       ∨ (c₁ = skip₁ ∧ et = (c₂, s))) :=
   propext {
     mp := λ h => match h with
@@ -41,49 +42,49 @@ theorem cat_eq:
   }
 
 theorem cond_eq:
-  (if b then c else d end, s) ⇒ ss
-    = (b⇓s ∧ ss = (c, s) ∨ b⇓s = false ∧ ss = (d, s)) :=
+  ((if b then c else d end, s) ⇒ ss)
+    = (b s ∧ ss = (c, s) ∨ b s = false ∧ ss = (d, s)) :=
   propext {
-    mp := λ h => match hb: b⇓s with
+    mp := λ h => match hb: b s with
       | false => match h with | step.ifₛ => Or.inr ⟨rfl, hb ▸ rfl⟩
       | true => match h with | step.ifₛ => Or.inl ⟨rfl, hb ▸ rfl⟩,
     mpr := λ h =>
-      let hss: ss = (bif b⇓s then c else d, s) :=
-        match hb: b⇓s with
+      let hss: ss = (bif b s then c else d, s) :=
+        match hb: b s with
         | true => match hb ▸ h with | Or.inl h => h.2
         | false => match hb ▸ h with | Or.inr h => h.2
       hss ▸ step.ifₛ
   }
 
-theorem cond_false {b: Bexp} (hb: b⇓s = false):
-  (if b then c else d end, s) ⇒ ss = (ss = (d, s)) :=
+theorem cond_false {b: Bexp} (hb: b s = false):
+  ((if b then c else d end, s) ⇒ ss) = (ss = (d, s)) :=
   propext {
     mp := λ h => match hb ▸ cond_eq ▸ h with
       | Or.inr ⟨_, h2⟩ => h2,
     mpr := λ h => cond_eq ▸ Or.inr ⟨hb, h⟩
   }
 
-infix:110 " ⇒* " => RTL step
+infixl:10 " ⇒* " => RTL step
 
 theorem star.demo₂:
-  (⦃x = 2; while 0 <= x loop x = x + 1 end⦄, σ₀) ⇒*
-      (⦃while 0 <= x loop x = x + 1 end⦄, σ₀⟪"x" ≔ 2⟫) :=
+  (⦃x = 2; while 0 <= x loop x = x + 1 end⦄, s₀) ⇒*
+      (⦃while 0 <= x loop x = x + 1 end⦄, s₀["x" ← 2]) :=
   RTL.head (step.catₙₛ step.assₛ) (RTL.head step.cat₀ₛ RTL.refl)
 
 theorem star.cat_skip_cat
   (h: (c, s) ⇒* (skip, t)):
-  (c;;d, s) ⇒* (skip;;d, t) :=
-  RTL.lift (λ (x: Com × State) => (x.1;;d, x.2)) (λ _ _ h => step.catₙₛ h) h
+  (c++d, s) ⇒* (skip++d, t) :=
+  RTL.lift (λ (x: Com × State) => (x.1++d, x.2)) (λ _ _ h => step.catₙₛ h) h
 
 theorem star.cat
   (h1: (c₁, s) ⇒* (skip₁, s₁))
   (h2: (c₂, s₁) ⇒* (skip₁, s₂)):
-  (c₁;;c₂, s) ⇒* (skip₁, s₂) :=
+  (c₁++c₂, s) ⇒* (skip₁, s₂) :=
   RTL.trans (cat_skip_cat h1) (RTL.trans (RTL.single step.cat₀ₛ) h2)
 
 theorem star.cat_no_influence
   (h: (c₁, s) ⇒* (skip₁, s₁)):
-  (c₁;;c₂, s) ⇒* (c₂, s₁) :=
+  (c₁++c₂, s) ⇒* (c₂, s₁) :=
   RTL.trans (cat_skip_cat h) (RTL.single step.cat₀ₛ)
 
 end Structural
